WIP on moving binencoders to ByteString.

src/BinEncoders/Env/BinLib/Core.v
@@ -1,4 +1,9 @@
 Require Import
+        Bedrock.Word
+        Coq.NArith.NArith
+        Coq.Arith.Arith
+        Coq.Numbers.Natural.Peano.NPeano
+        Coq.Logic.Eqdep_dec
         Fiat.BinEncoders.Env.Common.Specs.
 
 Set Implicit Arguments.
@@ -13,3 +18,720 @@ Global Instance btransformer : Transformer bin :=
      transform_id_left := @app_nil_l _;
      transform_id_right := @app_nil_r _;
      transform_assoc := @app_assoc _ |}.
+
+Definition char := word 8.
+
+Definition char_get_bit
+           (i : nat)
+           (c : word i)
+  := Nmod2 (Ndiv (wordToN c) (Npow2 i)).
+
+Definition char_set_bit (* Assumes the ith bit of c is unset. *)
+           (b : bool)
+           (i : nat)
+           (c : char) :=
+  if b then
+    wplus c (NToWord _ (Npow2 i))
+  else c.
+
+Definition char_chomp_bits
+           (i : word 3)
+           (c : char)
+  : word 7 :=
+  NToWord _ (N.modulo (wordToN c) (Npow2 (wordToNat i))).
+
+Record ByteString :=
+  { padding : nat; (* The number of valid bits in front. *)
+    paddingOK : lt padding 8;
+    front : word padding;
+    byteString : list char (* The bytestring. *)
+  }.
+
+Definition ByteString_push
+         (b : bool)
+         (bs : ByteString)
+  : ByteString.
+  refine (if (eq_nat_dec (padding bs) 7) then
+    {| front := (wzero _);
+       byteString := WS b _
+                        :: byteString bs;
+       padding := 0 |}
+  else
+    {| front := WS b (front bs);
+       byteString := byteString bs |}).
+  abstract omega.
+  pose (front bs) as w; destruct _H; exact w.
+  abstract (pose proof (paddingOK bs); omega).
+Defined.
+
+Definition ByteString_pop
+         (bs : ByteString)
+  : option (bool * ByteString).
+  refine (match padding bs as n return
+                word n
+                -> lt n 8
+                -> _ with
+          | 0 => fun _ _ =>
+                   match byteString bs with
+                   | [ ] =>  None
+                   | c :: l' => Some (whd c,
+                                      {| front := wtl c;
+                                         byteString := l' |})
+                   end
+          | S n => fun c lt_n => Some (whd c,
+                                  {| front := wtl c;
+                                     byteString := byteString bs |})
+          end (front bs) (paddingOK bs)).
+  abstract omega.
+  abstract omega.
+Defined.
+
+Fixpoint ByteString_push_word
+           {n}
+           (w : word n)
+           (bs : ByteString) :=
+  match w with
+  | WO => bs
+  | WS b _ w' => ByteString_push b (ByteString_push_word w' bs)
+  end.
+
+Definition ByteString_push_char (c : char) (bs : ByteString)
+  := ByteString_push_word c bs.
+
+Fixpoint ByteString_push_front
+           {n}
+           (w : word n)
+           (bs : ByteString) :=
+  match n return word n -> ByteString with
+  | 0 => fun _ => bs
+  | S n' => fun w =>
+              ByteString_push (whd w) (ByteString_push_front (wtl w) bs)
+  end w.
+
+Definition ByteString_transformer
+           (bs bs' : ByteString)
+  : ByteString :=
+  let bs'' := fold_right ByteString_push_char bs' (byteString bs) in
+  ByteString_push_front (front bs) bs''.
+
+Definition length_ByteString (bs : ByteString) :=
+  (padding bs) + (8 * (length (byteString bs))).
+
+Lemma length_ByteString_push
+  : forall (bs' : ByteString)
+           (b : bool),
+    length_ByteString (ByteString_push b bs') =
+    S (length_ByteString bs').
+Proof.
+  simpl; clear; destruct bs'; simpl.
+  unfold ByteString_push; simpl.
+  destruct (eq_nat_dec padding0 7);
+    intros; simpl; subst.
+  - unfold length_ByteString; simpl; omega.
+  - unfold length_ByteString; simpl; omega.
+Qed.
+
+Lemma length_ByteString_push_char
+  : forall (bs' : ByteString)
+           (c : char),
+    length_ByteString (ByteString_push_char c bs') =
+    8 + (length_ByteString bs').
+Proof.
+  intros.
+  pose proof (shatter_word c); simpl in *;
+    pose proof (shatter_word (wtl c)); simpl in *;
+      pose proof (shatter_word (wtl (wtl c))); simpl in *;
+        pose proof (shatter_word (wtl (wtl (wtl c)))); simpl in *;
+          pose proof (shatter_word (wtl (wtl (wtl (wtl c))))); simpl in *;
+            pose proof (shatter_word (wtl (wtl (wtl (wtl (wtl c)))))); simpl in *;
+              pose proof (shatter_word (wtl (wtl (wtl (wtl (wtl (wtl c))))))); simpl in *;
+                pose proof (shatter_word (wtl (wtl (wtl (wtl (wtl (wtl (wtl c))))))));
+                pose proof (shatter_word (wtl (wtl (wtl (wtl (wtl (wtl (wtl (wtl c))))))))); simpl in *.
+  rewrite H, H0, H1, H2, H3, H4, H5, H6, H7; simpl.
+  unfold ByteString_push_char; simpl.
+  rewrite !length_ByteString_push; repeat f_equal.
+Qed.
+
+Lemma length_ByteString_append
+  : forall bs (bs' : ByteString),
+    length_ByteString (fold_right ByteString_push_char bs' bs)
+    = (8 * (length bs)) + length_ByteString bs'.
+Proof.
+  induction bs; eauto.
+  simpl length; rewrite mult_succ_r, plus_comm.
+  intros; rewrite <- plus_assoc, <- IHbs.
+  simpl; rewrite length_ByteString_push_char.
+  omega.
+Qed.
+
+Corollary length_ByteString_push_front
+  : forall n (bs_front : word n) (bs' : ByteString),
+    length_ByteString (ByteString_push_front bs_front bs') =
+    n + length_ByteString bs'.
+Proof.
+  induction n; simpl; intros; eauto.
+  rewrite length_ByteString_push, IHn; eauto.
+Qed.
+
+Lemma transform_ByteString_measure
+  : forall bs bs' : ByteString,
+   length_ByteString (ByteString_transformer bs bs') = length_ByteString bs + length_ByteString bs'.
+Proof.
+  destruct bs as [bs_padding bs_front ? bs_byteString]; simpl.
+  induction bs_byteString.
+  - unfold ByteString_transformer, length_ByteString at 2; simpl.
+    rewrite NPeano.Nat.add_0_r.
+    induction bs_padding.
+    + simpl; eauto.
+    + simpl; intros.
+      rewrite length_ByteString_push; rewrite IHbs_padding; eauto.
+      omega.
+  -  unfold ByteString_transformer in *; simpl in *.
+     unfold length_ByteString at 2.
+     unfold byteString at 1.
+     intros; rewrite <- plus_assoc,
+             <- (length_ByteString_append (a :: bs_byteString) bs').
+     simpl fold_right.
+     rewrite length_ByteString_push_char, plus_comm.
+     rewrite <- plus_assoc.
+     simpl padding.
+     unfold length_ByteString in IHbs_byteString.
+     simpl byteString in IHbs_byteString.
+     simpl padding in IHbs_byteString.
+     rewrite length_ByteString_append.
+     unfold length_ByteString at 2.
+     replace (8 * length bs_byteString +
+              (padding bs'
+               + 8 * length (byteString bs'))
+              + bs_padding) with
+     (bs_padding + 8 * length bs_byteString +
+      (padding bs' + 8 * length (byteString bs'))) by omega.
+     rewrite <- IHbs_byteString; clear.
+     rewrite !length_ByteString_push_front.
+     rewrite length_ByteString_push_char, plus_comm, plus_assoc.
+     rewrite <- !plus_assoc; f_equal.
+     remember (fold_right ByteString_push_char bs' bs_byteString);
+       clear.
+     induction bs_padding.
+     + unfold length_ByteString; simpl; omega.
+     + rewrite <- plus_n_Sm, (IHbs_padding (wtl front0)); clear.
+       rewrite plus_n_Sm.
+       simpl ByteString_push_front.
+       destruct (ByteString_push_front (wtl front0) y) eqn: ?.
+       unfold ByteString_push.
+       destruct (eq_nat_dec (padding (ByteString_push_front (wtl front0) y)) 7);
+         simpl padding; simpl byteString.
+       * simpl length; rewrite Heqb; simpl byteString;
+           rewrite Heqb in e; simpl in e.
+         rewrite e; omega.
+       * rewrite Heqb in n; rewrite Heqb;
+           simpl padding in *; simpl byteString in *; clear Heqb.
+         omega.
+Qed.
+
+Definition ByteString_id : ByteString.
+  refine {| front := WO; byteString := [] |}.
+  abstract omega.
+Defined.
+
+Lemma ByteString_transform_id_left
+  : forall bs : ByteString,
+   ByteString_transformer ByteString_id bs = bs.
+Proof.
+  reflexivity.
+Qed.
+
+(* Uniqueness of less than proofs taken from *)
+(* https://coq.inria.fr/faq#le-uniqueness. *)
+Scheme le_ind' := Induction for le Sort Prop.
+Theorem le_uniqueness_proof : forall (n m : nat) (p q : le n m), p = q.
+Proof.
+  induction p using le_ind'; intro q.
+  replace (le_n n) with
+  (eq_rect _ (fun n0 => le n n0) (le_n n) _ (refl_equal n)).
+  2:reflexivity.
+  generalize (refl_equal n).
+  pattern n at 2 4 6 10, q; case q; [intro | intros m l e].
+  rewrite <- (eq_rect_eq_dec eq_nat_dec); eauto.
+  contradiction (le_Sn_n m); rewrite <- e; assumption.
+  replace (le_S n m p) with
+  (eq_rect _ (fun n0 => le n n0) (le_S n m p) _ (refl_equal (S m))).
+  2:reflexivity.
+  generalize (refl_equal (S m)).
+  pattern (S m) at 1 3 4 6, q; case q; [intro Heq | intros m0 l HeqS].
+  contradiction (le_Sn_n m); rewrite Heq; assumption.
+  injection HeqS; intro Heq; generalize l HeqS.
+  rewrite <- Heq; intros; rewrite <- (eq_rect_eq_dec eq_nat_dec).
+  rewrite (IHp l0); reflexivity.
+Qed.
+
+Fixpoint append_word {n m}
+           (w : word n)
+           (w' : word m)
+  : word (n + m) :=
+  match n return word n -> word (n + m) with
+  | 0 => fun _ => w'
+  | S n' => fun w => WS (whd w) (append_word (wtl w) w')
+  end w.
+
+Lemma minus_inj
+  : forall m m' y q q',
+    (q < y)%nat
+    -> (q' < y)%nat
+    -> (m * y) + y - q = (m' * y) + y - q'
+    -> m = m' /\ q = q'.
+Proof.
+  induction m; simpl; intros.
+  - destruct m'.
+    + simpl in *; intuition.
+    + rewrite mult_succ_l in *.
+      assert (y - q < (m' * y) + y + y - q')%nat.
+      { clear H1; induction (m' * y); intros.
+        - omega.
+        - etransitivity.
+          apply IHn.
+          omega. }
+      elimtype False.
+      rewrite H1 in H2.
+      omega.
+  - destruct m'.
+    + simpl in *.
+      assert (y - q' < (m * y) + y + y - q)%nat.
+      { clear H1 IHm; induction (m * y); intros.
+        - omega.
+        - etransitivity.
+          apply IHn.
+          omega. }
+      elimtype False.
+      rewrite <- H1 in H2; omega.
+    + destruct (IHm m' _ _ _ H H0).
+      simpl in H1.
+      rewrite <- !Nat.add_sub_assoc in H1; try omega.
+      subst; intuition.
+Qed.
+
+Corollary minus_inj'
+  : forall m m' y q q',
+    (q <= y)%nat
+    -> (q' <= y)%nat
+    -> m * (S y) + y - q = (m' * (S y)) + y - q'
+    -> m = m' /\ q = q'.
+Proof.
+  intros; destruct (@minus_inj m m' (S y) q q'); try omega.
+  assert (m * S y + S y - q = S (m * S y + y - q)).
+  rewrite plus_comm.
+  assert (S y + m * S y - q = 1 + (y + m * S y - q)).
+  rewrite !Nat.add_sub_assoc.
+  rewrite plus_assoc.
+  omega.
+  auto with arith.
+  rewrite H2; simpl; omega.
+  rewrite H2.
+  rewrite H1.
+  rewrite <- !Nat.add_sub_assoc; auto.
+  omega.
+Qed.
+
+Lemma divmod_eq' :
+  forall x y q u,
+    (u <= y)%nat
+    -> x = q * (S y) + (y - u)
+    -> divmod x y 0 y = (q, u).
+Proof.
+  intros; pose proof (divmod_spec x y 0 y).
+  destruct (divmod x y 0 y); destruct H1; eauto.
+  rewrite H0 in H1.
+  simpl in H1.
+  rewrite minus_diag, <- mult_n_O, <- !plus_n_O in *.
+  assert (n + y * n = n * S y) by
+      (rewrite mult_succ_r, plus_comm, mult_comm; reflexivity).
+  f_equal; eapply (@minus_inj' n q y n0 u); eauto;
+  rewrite !mult_succ_r in *;
+  rewrite !Nat.add_sub_assoc in H1; eauto;
+      omega.
+Qed.
+
+Lemma divmod_eq :
+  forall x y q u,
+    divmod x y 0 y = (q, u) ->
+    x = q * (S y) + (y - u).
+Proof.
+  intros; pose proof (divmod_spec x y 0 y).
+  rewrite H in H0; destruct H0; eauto.
+  simpl in H0.
+  assert (x = q + y * q + (y - u)) by omega.
+  rewrite H2.
+  rewrite mult_succ_r.
+  rewrite (plus_comm (q * y) q).
+  rewrite mult_comm; f_equal.
+Qed.
+
+Lemma NatModulo_S_Full
+  : forall n' m, Nat.modulo n' (S m) = m
+               -> Nat.modulo (S n') (S m) = 0.
+Proof.
+  unfold Nat.modulo, modulo.
+  intros; assert (exists q, divmod (S n') m 0 m = (q, m)).
+  intros; pose proof (divmod_spec n' m 0 m).
+  destruct (divmod n' m 0 m) eqn: ? .
+  destruct H0; eauto.
+  simpl in H.
+  assert (n0 = 0) by omega.
+  rewrite H2 in *; clear H H2.
+  apply divmod_eq in Heqp.
+  eexists (S n).
+  eapply divmod_eq'; eauto.
+  rewrite Heqp.
+  rewrite <- !minus_n_O, minus_diag, <- plus_n_O.
+  simpl; omega.
+  destruct_ex; rewrite H0; simpl; omega.
+Qed.
+
+Lemma NatModulo_S_Not_Full
+  : forall n' m, Nat.modulo n' (S m) <> m
+               -> Nat.modulo (S n') (S m) = S (Nat.modulo n' (S m)).
+Proof.
+  unfold Nat.modulo, modulo.
+  intros; destruct (divmod n' m 0 m) eqn: ?.
+  destruct n0.
+  simpl in H; omega.
+  intros; pose proof (divmod_spec n' m 0 m).
+  rewrite Heqp in H0; destruct H0; eauto.
+  assert (divmod (S n') m 0 m = (n, n0)).
+  apply divmod_eq in Heqp.
+  apply divmod_eq'; try omega.
+  rewrite H2; simpl.
+  omega.
+Qed.
+
+Fixpoint word_into_char {n}
+           (w : word n)
+           {struct w}
+  : (word (Nat.modulo n 8) * list char).
+  refine (match w in word n return word (Nat.modulo n 8) * list char with
+          | WO => (WO, [ ])
+          | WS b n' w' => let (b', chars) := word_into_char _ w' in
+                          (if (eq_nat_dec (Nat.modulo n' 8) 7) then _
+                                                else (_ , chars))
+          end).
+  - generalize (WS b b'); rewrite _H, (NatModulo_S_Full _ _H); simpl.
+    exact (fun b => (WO, b :: chars)).
+  - rewrite (NatModulo_S_Not_Full _ _H).
+    exact (WS b b').
+Defined.
+
+(*Lemma ByteString_push_front_eq
+  : forall bs {n} (w : word n) pf,
+    ByteString_push_front w bs =
+    {| front := fst (word_into_char (append_word w (front bs)));
+       paddingOK := pf;
+       byteString := snd (word_into_char (append_word w (front bs)))
+                         ++ byteString bs|}.
+Proof.
+  destruct bs; simpl front; simpl byteString; simpl padding.
+  induction w.
+Admitted.
+  Focus 2.
+  simpl ByteString_push_front.
+  cbv beta.
+  simpl wtl; simpl whd.
+  intro. erewrite IHw.
+  unfold ByteString_push.
+  - simpl; intros.
+    assert (word_into_char front0 = (front0, [ ])).
+    assert (match snd (divmod padding0 7 0 7) with
+              | 0 => 7
+              | 1 => 6
+              | 2 => 5
+              | 3 => 4
+              | 4 => 3
+              | 5 => 2
+              | 6 => 1
+              | S (S (S (S (S (S (S _)))))) => 0
+              end = padding0).
+    Focus 2.
+    revert pf. rewrite H.
+    induction front0.
+    + simpl; f_equal; apply le_uniqueness_proof.
+    + assert (S n =
+              match snd (divmod (S n) 7 0 7) with
+              | 0 => 7
+              | 1 => 6
+              | 2 => 5
+              | 3 => 4
+              | 4 => 3
+              | 5 => 2
+              | 6 => 1
+              | S (S (S (S (S (S (S _)))))) => 0
+              end).
+      Focus 2.
+      revert front0 paddingOK0 pf IHfront0.
+      rewrite <- H.
+      rewrite (@divmod_eq' (S n) 7 0 (S n)).
+
+  f_equal.
+Admitted. *)
+
+Lemma ByteString_push_char_id_right
+  : forall (chars : list char) (bs : ByteString),
+    padding bs = 0 ->
+    fold_right ByteString_push_char bs chars =
+    {| front := WO;
+       paddingOK := ByteString_id_subproof;
+       byteString := chars ++ (byteString bs) |}.
+Proof.
+  (* Commented out because the proof is slow and takes a bunch of memory. *)
+  (*
+  destruct bs; simpl; intros; subst.
+  induction chars; simpl.
+  - f_equal; eauto using le_uniqueness_proof.
+  - rewrite IHchars.
+    rename a into c.
+    pose proof (shatter_word c); simpl in *;
+    pose proof (shatter_word (wtl c)); simpl in *;
+      pose proof (shatter_word (wtl (wtl c))); simpl in *;
+        pose proof (shatter_word (wtl (wtl (wtl c)))); simpl in *;
+          pose proof (shatter_word (wtl (wtl (wtl (wtl c))))); simpl in *;
+            pose proof (shatter_word (wtl (wtl (wtl (wtl (wtl c)))))); simpl in *;
+              pose proof (shatter_word (wtl (wtl (wtl (wtl (wtl (wtl c))))))); simpl in *;
+                pose proof (shatter_word (wtl (wtl (wtl (wtl (wtl (wtl (wtl c))))))));
+                pose proof (shatter_word (wtl (wtl (wtl (wtl (wtl (wtl (wtl (wtl c))))))))); simpl in *.
+  rewrite H, H0, H1, H2, H3, H4, H5, H6, H7; simpl.
+  unfold ByteString_push_char; simpl.
+  repeat match goal with
+    |- context [(whd ?c)] => destruct (whd c) end;
+    try solve [compute; f_equal; eapply le_uniqueness_proof].
+Qed. *)
+Admitted.
+
+Lemma ByteString_transform_id_right
+  : forall bs : ByteString,
+    ByteString_transformer bs ByteString_id = bs.
+Proof.
+  destruct bs; unfold ByteString_transformer, ByteString_id; simpl.
+  rewrite ByteString_push_char_id_right; simpl; eauto.
+  rewrite app_nil_r.
+  induction front0.
+  + simpl; f_equal.
+    pose ByteString_id_subproof.
+    eapply le_uniqueness_proof.
+  + simpl.
+    assert (lt n 8) by omega.
+    erewrite (IHfront0 H).
+    unfold ByteString_push.
+    simpl.
+    destruct (eq_nat_dec n 7); subst.
+    omega.
+    f_equal; eauto using le_uniqueness_proof.
+Qed.
+
+Lemma ByteString_transform_f_equal
+  : forall bs bs'
+           (p_eq : padding bs' = padding bs),
+    paddingOK bs = (@eq_rect nat (padding bs') (fun t => lt t 8) (paddingOK bs') _ p_eq)
+    -> front bs = (@eq_rect nat (padding bs') (fun t => word t) (front bs') _ p_eq)
+    -> byteString bs = byteString bs'
+    -> bs = bs'.
+Proof.
+  destruct bs; destruct bs'; simpl.
+  intros; subst; reflexivity.
+Qed.
+
+(*Lemma padding_ByteString_transform_assoc
+  : forall l m n : ByteString,
+    padding (ByteString_transformer l (ByteString_transformer m n)) =
+    padding (ByteString_transformer (ByteString_transformer l m) n).
+Proof.
+  intros; repeat (erewrite ByteString_transformer_eq; simpl padding).
+Admitted. *)
+
+Lemma ByteString_transform_assoc
+  : forall l m n : ByteString,
+    ByteString_transformer l (ByteString_transformer m n) =
+    ByteString_transformer (ByteString_transformer l m) n.
+Proof.
+(*
+  revert bs_m padding_l front_l padding_m front_m
+         padding_l_OK padding_m_OK
+         padding_n padding_n_OK front_n bs_n.
+  induction bs_l; simpl.
+  - induction bs_m; simpl.
+    intros; erewrite !ByteString_push_front_eq.
+    assert (Nat.modulo
+                (padding_l +
+                 padding
+                   (ByteString_push_front front_m
+                      {|
+                      padding := padding_n;
+                      paddingOK := padding_n_OK;
+                      front := front_n;
+                      byteString := bs_n |})) 8
+            =  Nat.modulo
+                (padding
+                   (ByteString_push_front front_l
+                      {|
+                      padding := padding_m;
+                      paddingOK := padding_m_OK;
+                      front := front_m;
+                      byteString := [] |}) +
+                 padding
+                   (fold_right ByteString_push_char
+                      {|
+                      padding := padding_n;
+                      paddingOK := padding_n_OK;
+                      front := front_n;
+                      byteString := bs_n |}
+                      (byteString
+                         (ByteString_push_front front_l
+                            {|
+                            padding := padding_m;
+                            paddingOK := padding_m_OK;
+                            front := front_m;
+                            byteString := [] |})))) 8).
+    admit.
+    rewrite H.
+    apply f_equal.
+    repeat f_equal.
+    + induction front_l; simpl.
+      * reflexivity.
+      * intros; erewrite !ByteString_push_front_eq.
+        simpl.
+    + reflexivity.
+    + simpl. *)
+Admitted.
+
+Global Instance ByteStringTransformer : Transformer ByteString :=
+  {| transform := ByteString_transformer;
+     bin_measure := length_ByteString;
+     transform_measure := transform_ByteString_measure;
+     transform_id := ByteString_id;
+     transform_id_left := ByteString_transform_id_left;
+     transform_id_right := ByteString_transform_id_right;
+     transform_assoc :=  ByteString_transform_assoc |}.
+
+Lemma ByteString_measure_push
+  : forall (t : bool) (b : ByteString), bin_measure (ByteString_push t b) = bin_measure b + 1.
+Proof.
+  destruct b; unfold ByteString_push, length_ByteString; simpl.
+  unfold length_ByteString; simpl.
+  destruct (eq_nat_dec padding0 7); simpl.
+  - rewrite e; simpl; omega.
+  - omega.
+Qed.
+
+Lemma ByteString_measure_pop_Some
+  : forall (b' : ByteString) (t : bool) (b : ByteString),
+    ByteString_pop b = Some (t, b') -> bin_measure b = bin_measure b' + 1.
+Proof.
+  destruct b.
+  unfold ByteString_pop; simpl.
+  destruct padding0.
+  - destruct byteString0.
+    + intros; discriminate.
+    + intros; injections.
+      unfold length_ByteString; simpl.
+      omega.
+  - intros; injections.
+    unfold length_ByteString; simpl.
+    omega.
+Qed.
+
+Lemma ByteString_transform_push_pop_opt
+  : forall (t : bool) (m : ByteString), ByteString_pop (ByteString_push t m) = Some (t, m).
+Proof.
+  destruct m; simpl.
+  unfold ByteString_push; unfold ByteString_pop.
+  simpl padding.
+  destruct (eq_nat_dec padding0 7);
+    simpl padding; simpl paddingOK; simpl front; simpl byteString.
+  - subst; simpl; repeat f_equal.
+    apply le_uniqueness_proof.
+  - simpl; repeat f_equal.
+    apply le_uniqueness_proof.
+Qed.
+
+Lemma ByteString_transform_push_eq
+  : forall t bs, exists pf,
+      ByteString_push t bs = transform {| front := WS t WO;
+                                         paddingOK := pf;
+                                         byteString := [ ] |} bs.
+Proof.
+  assert (1 < 8)%nat by omega.
+  intros; eexists H.
+  destruct bs; simpl.
+  reflexivity.
+Qed.
+
+Lemma ByteString_transform_push_step_opt
+  : forall (t : bool) (m n : ByteString),
+    transform (ByteString_push t m) n = ByteString_push t (transform m n).
+Proof.
+  intros; destruct (ByteString_transform_push_eq t m).
+  simpl transform.
+  rewrite H, <- ByteString_transform_assoc.
+  destruct (ByteString_transform_push_eq t (transform m n)).
+  simpl transform in *; rewrite H0.
+  repeat f_equal.
+  apply le_uniqueness_proof.
+Qed.
+
+Lemma ByteString_transform_pop_opt_inj
+  : forall (t : bool) (m b b' : ByteString),
+    ByteString_pop b = Some (t, m) -> ByteString_pop b' = Some (t, m) -> b = b'.
+Proof.
+  destruct b; destruct b'.
+  unfold ByteString_pop;
+    simpl padding; simpl paddingOK; simpl front; simpl byteString.
+  destruct padding0; destruct padding1.
+  - destruct byteString0; intros; try discriminate.
+    destruct byteString1; try discriminate.
+    injection H; injection H0; intros.
+    subst.
+    f_equal.
+    apply le_uniqueness_proof.
+    rewrite (shatter_word_0 front0);
+      rewrite (shatter_word_0 front1); reflexivity.
+    rewrite (shatter_word c) in *;
+      rewrite (shatter_word c0) in *.
+    injection H3; intros.
+    rewrite H1; f_equal.
+    f_equal.
+    simpl in H4; rewrite H4; reflexivity.
+    apply inj_pair2_eq_dec in H2; eauto.
+    apply eq_nat_dec.
+  - destruct byteString0; intros; try discriminate.
+    injection H; injection H0; intros.
+    rewrite <- H1 in H3; injection H3; intros.
+    elimtype False.
+    generalize H7 paddingOK1; clear; intro; rewrite H7.
+    intros; omega.
+  - destruct byteString1; intros; try discriminate.
+    injection H; injection H0; intros.
+    rewrite <- H1 in H3; injection H3; intros.
+    elimtype False.
+    generalize H7 paddingOK0; clear; intro; rewrite H7.
+    intros; omega.
+  - intros; injection H; injection H0; intros.
+    rewrite <- H1 in H3; injection H3; intros; subst.
+    repeat f_equal.
+    apply le_uniqueness_proof.
+    rewrite (shatter_word front0); rewrite (shatter_word front1);
+      f_equal; eauto.
+    apply inj_pair2_eq_dec in H6; eauto.
+    apply eq_nat_dec.
+Qed.
+
+Instance ByteString_TransformerUnitOpt
+  : TransformerUnitOpt ByteStringTransformer bool :=
+  {| T_measure f := 1;
+     transform_push_opt := ByteString_push;
+     transform_pop_opt := ByteString_pop;
+     measure_push := ByteString_measure_push ;
+     measure_pop_Some := ByteString_measure_pop_Some;
+     transform_push_pop_opt := ByteString_transform_push_pop_opt;
+     transform_push_step_opt := ByteString_transform_push_step_opt;
+     transform_pop_opt_inj := ByteString_transform_pop_opt_inj
+  |}.
+Proof.
+  - abstract eauto.
+Defined.
